---
title: "SRout Assign 14"
date: 11/25/2020
output:
  pdf_document: default
  prettydoc::html_pretty: 
    theme: architect
  html_document: default
---

```{r setup, include=FALSE}
knitr::opts_chunk$set(echo = TRUE)
```

<span style="color:green"> **
This week, we'll work out some Taylor Series expansions of popular functions.**</span>


* <span style="color:green">**1. f(x) = $\frac {1}{1-x}$**</span>


<span style="color:darkred">**Solution**</span>

$$f(x) = \frac {1}{1-x}$$
Formula for a Taylor Series Expansion:
$$f(x) = \sum_{n=0} ^ {\infty} \frac {f^{(n)}(a)}{n!} (x - a) ^ {n}$$
$$f(x)= f(a) + f'(a)(x-a) + \frac {f''(a)}{2!}(x-a)^2 + \frac {f'''(a)}{3!}(x-a)^3 + \frac {f''''(a)}{4!}(x-a)^4 + ........$$
Derivatives of first order, second order, third order and fourth order of f(x) shown below:

$$f(x) =  \frac {1}{1-x}, f(0) = \frac {1} {1-0} = 1$$
$$f'(x) =  \frac {1}{(1-x)^2}, f'(0) = \frac {1} {(1-0)^2} = 1$$
$$f''(x) =  \frac {2}{(1-x)^3}, f''(0) = \frac {2} {(1-0)^3} = 2$$
$$f'''(x) =  \frac {6}{(1-x)^4}, f'''(0) = \frac {6} {(1-0)^4} = 6$$
$$f''''(x) =  \frac {24}{(1-x)^5}, f''''(0) = \frac {24} {(1-0)^5} = 24$$
if we do till, $$f^n(x) = \frac {n!}{(1-x)^{(n+1)}}$$

Substitute expressions into Taylor Series expansion:

$$f(x) = 1 + \frac {1}{1!}x^1 + \frac {2}{2!}x^2 + \frac {6}{3!}x^3 + \frac {24}{4!}x^4 + .....+ \frac {n!}{n!}x^n$$
$$f(x) = \sum_{n = 0}^{\infty}x^n$$

* <span style="color:green">**2. f(x) = e^x <br>**</span>

<span style="color:darkred">**Solution**</span>

$$f(x) = e^x$$
$$f'(x) = e^x, f'(0) = e^0 = 1$$
$$f''(x) = e^x , f''(0) = e^0 = 1$$
$$f'''(x) = e^x , f'''(0) = e^0 = 1$$
$$.....$$

$$f^{(n)}(x) = e^x  , f^n(0) = e^0 = 1$$
Substitute expressions into Taylor Series expansion:

$$f(x) = \sum_{n=0}^{\infty} \frac {f^{(n)}(a)}{n!} (x - a) ^ {n}$$

$$f(x) = e^0 + e^0(x-0) + e^0(x-0)^2 + e^0(x-0)^3 + ...... + e^0(x-0)^n$$

$$f(x) = 1 + x + \frac {x^2}{2!} + \frac {x^3}{3!} + \frac {x^4}{4!} + ......+ \frac {x^n}{n!}$$

$$f(x) = \sum_{n=0}^{\infty} \frac {1}{n!}x^n$$

$$f(x) = \sum_{n=0}^{\infty} \frac {x^n} {n!}$$

* <span style="color:green">**3. f(x) = ln(1 + x) <br>**</span>

<span style="color:darkred">**Solution**</span>

$$f(x) = ln(1 + x), f(0) = 0$$
$$f'(x) = \frac {1}{1+x}, f'(0) = 1$$

$$f''(x) = \frac {-1}{(1+x)^2}, f''(0) = -1$$
$$f'''(x) = \frac {2}{(1+x)^3}, f'''(0) = 2$$

$$f''''(x) = \frac {-6}{(1+x)^4}, f'''(0) = -6$$
$$......$$

$$f^n(x) = \frac {(-1) ^{(n-1)}(n-1)!} {(x+1)^n}, f^n(0) = (-1) ^{(n-1)}(n-1)!$$

Substitute expressions into Taylor Series expansion:

$$f(x) = f(0) + f'(0)(x-0) + \frac {f''(0)}{2!}(x-0)^2 + \frac {f'''(0)}{3!}(x-0)^3 + \frac {f''''(0)}{4!}(x-0)^4 + ........$$

$$f(x) = 0 + x - \frac {1}{2}x^2 + \frac{1}{3}x^3 - \frac {1}{4}x^4+ ......$$

$$f(x) = \sum_{n=1}^{\infty} \frac {(-1) ^{(n-1)}(n-1)!} {n!} (x)^n$$

